add support for unknown expressions in programs

theories/simplang/tactics.v
@@ -1,5 +1,5 @@
-From simuliris.simplang Require Import lang.
 From stdpp Require Import fin_maps.
+From simuliris.simplang Require Import lang parallel_subst notation.
 
 
 (** The tactic [reshape_expr e tac] decomposes the expression [e] into an
@@ -63,3 +63,368 @@ Global Hint Extern 0 (head_reducible _ _ _) => eexists _, _, _; simpl : head_ste
 Global Hint Extern 1 (head_step _ _ _ _ _ _) => econstructor : head_step.
 (*Global Hint Extern 0 (head_step _ (CmpXchg _ _ _) _ _ _ _) => eapply CmpXchgS : head_step.*)
 Global Hint Extern 0 (head_step _ (AllocN _ _) _ _ _ _) => apply alloc_fresh : head_step.
+
+Module W.
+  Inductive expr :=
+  | Expr (e : simp_lang.expr)
+  | ClosedExpr (f : list string) (e : simp_lang.expr) (Hfree : (free_vars e) = list_to_set f)
+  | SubstMap (xs : list (string * val)) (e : expr)
+
+  | Val (v : val)
+  | Var (x : string)
+  | Let (x : binder) (e1 e2 : expr)
+  | Call (e1 : expr) (e2 : expr)
+  | UnOp (op : un_op) (e : expr)
+  | BinOp (op : bin_op) (e1 e2 : expr)
+  | If (e0 e1 e2 : expr)
+  | While (e0 e1 : expr)
+  | Pair (e1 e2 : expr)
+  | Fst (e : expr)
+  | Snd (e : expr)
+  | InjL (e : expr)
+  | InjR (e : expr)
+  | Match (e0 : expr) (x1 : binder) (e1 : expr) (x2 : binder) (e2 : expr)
+  | Fork (e : expr)
+  | AllocN (e1 e2 : expr)
+  | FreeN (e1 e2 : expr)
+  | Load (o : order) (e : expr)
+  | Store (o : order) (e1 : expr) (e2 : expr)
+  | CmpXchg (e0 : expr) (e1 : expr) (e2 : expr)
+  | FAA (e1 : expr) (e2 : expr)
+  .
+  Fixpoint to_expr (e : expr) : simp_lang.expr :=
+    match e with
+    | Expr e => e
+    | ClosedExpr f e Hfree => e
+    | SubstMap xs e => subst_map (list_to_map xs) (to_expr e)
+    | Val v => simp_lang.Val v
+    | Var x => simp_lang.Var x
+    | Let x e1 e2 => simp_lang.Let x (to_expr e1) (to_expr e2)
+    | Call e1 e2 => simp_lang.Call (to_expr e1) (to_expr e2)
+    | UnOp op e => simp_lang.UnOp op (to_expr e)
+    | BinOp op e1 e2 => simp_lang.BinOp op (to_expr e1) (to_expr e2)
+    | If e0 e1 e2 => simp_lang.If (to_expr e0) (to_expr e1) (to_expr e2)
+    | While e0 e1 => simp_lang.While (to_expr e0) (to_expr e1)
+    | Pair e1 e2 => simp_lang.Pair (to_expr e1) (to_expr e2)
+    | Fst e => simp_lang.Fst (to_expr e)
+    | Snd e => simp_lang.Snd (to_expr e)
+    | InjL e => simp_lang.InjL (to_expr e)
+    | InjR e => simp_lang.InjR (to_expr e)
+    | Match e0 x1 e1 x2 e2 => simp_lang.Match (to_expr e0) x1 (to_expr e1) x2 (to_expr e2)
+    | Fork e => simp_lang.Fork (to_expr e)
+    | AllocN e1 e2 => simp_lang.AllocN (to_expr e1) (to_expr e2)
+    | FreeN e1 e2 => simp_lang.FreeN (to_expr e1) (to_expr e2)
+    | Load o e => simp_lang.Load o (to_expr e)
+    | Store o e1 e2 => simp_lang.Store o (to_expr e1) (to_expr e2)
+    | CmpXchg e0 e1 e2 => simp_lang.CmpXchg (to_expr e0) (to_expr e1) (to_expr e2)
+    | FAA e1 e2 => simp_lang.FAA (to_expr e1) (to_expr e2)
+    end.
+
+  Ltac of_expr e :=
+  lazymatch e with
+
+  | subst_map ?xs ?e =>
+    let e := of_expr e in constr:(SubstMap (map_to_list xs) e)
+  | simp_lang.Val ?x => constr:(Val x)
+  | simp_lang.Var ?x => constr:(Var x)
+  | simp_lang.Let ?x ?e1 ?e2 =>
+    let e1 := of_expr e1 in let e2 := of_expr e2 in constr:(Let x e1 e2)
+  | simp_lang.Call ?e1 ?e2 =>
+    let e1 := of_expr e1 in let e2 := of_expr e2 in constr:(Call e1 e2)
+  | simp_lang.UnOp ?op ?e =>
+    let e := of_expr e in constr:(UnOp op e)
+  | simp_lang.BinOp ?op ?e1 ?e2 =>
+    let e1 := of_expr e1 in let e2 := of_expr e2 in constr:(BinOp op e1 e2)
+  | simp_lang.If ?e1 ?e2 ?e3 =>
+    let e1 := of_expr e1 in let e2 := of_expr e2 in let e3 := of_expr e3 in constr:(If e1 e2 e3)
+  | simp_lang.While ?e1 ?e2 =>
+    let e1 := of_expr e1 in let e2 := of_expr e2 in constr:(While e1 e2)
+  | simp_lang.Pair ?e1 ?e2 =>
+    let e1 := of_expr e1 in let e2 := of_expr e2 in constr:(Pair e1 e2)
+  | simp_lang.Fst ?e =>
+    let e := of_expr e in constr:(Fst e)
+  | simp_lang.Snd ?e =>
+    let e := of_expr e in constr:(Snd e)
+  | simp_lang.InjL ?e =>
+    let e := of_expr e in constr:(InjL e)
+  | simp_lang.InjR ?e =>
+    let e := of_expr e in constr:(InjR e)
+  | simp_lang.Match ?e1 ?x1 ?e2 ?x2 ?e3 =>
+    let e1 := of_expr e1 in let e2 := of_expr e2 in let e3 := of_expr e3 in constr:(Match e1 x1 e2 x2 e3)
+  | simp_lang.Fork ?e =>
+    let e := of_expr e in constr:(Fork e)
+  | simp_lang.AllocN ?e1 ?e2 =>
+    let e1 := of_expr e1 in let e2 := of_expr e2 in constr:(AllocN e1 e2)
+  | simp_lang.FreeN ?e1 ?e2 =>
+    let e1 := of_expr e1 in let e2 := of_expr e2 in constr:(FreeN e1 e2)
+  | simp_lang.Load ?o ?e =>
+    let e := of_expr e in constr:(Load o e)
+  | simp_lang.Store ?o ?e1 ?e2 =>
+    let e1 := of_expr e1 in let e2 := of_expr e2 in constr:(Store o e1 e2)
+  | simp_lang.CmpXchg ?e1 ?e2 ?e3 =>
+    let e1 := of_expr e1 in let e2 := of_expr e2 in let e3 := of_expr e3 in constr:(CmpXchg e1 e2 e3)
+  | simp_lang.FAA ?e1 ?e2 =>
+    let e1 := of_expr e1 in let e2 := of_expr e2 in constr:(FAA e1 e2)
+
+  | _ =>
+    lazymatch goal with
+    | H : free_vars e = list_to_set ?f |- _ =>
+      constr:(ClosedExpr f e H)
+    (*
+    | H : free_vars e = ?f |- _ =>
+      let rec go f :=
+          lazymatch f with
+          | {[ ?x ]} ∪ ?f' =>
+            let _ := match x with | _ => idtac x f' end in
+            let l := go f' in
+            let _ := match x with | _ => idtac x f' l end in
+            constr:(@cons string x l)
+          | {[ ?x ]} =>
+            constr:(@cons string x nil)
+          | ∅ =>
+            let _ := match f with | _ => idtac f  end in
+            constr:(@nil string)
+          end in
+      let l := go f in
+      (* idtac f; *)
+      let H' := fresh in
+      let _ := match f with | _ =>
+                              assert (free_vars e = list_to_set l) as H'; [admit|]
+               end in
+      constr:(ClosedExpr l e H')
+     *)
+    | _ => constr:(Expr e)
+    end
+  end.
+
+  Fixpoint subst (x : string) (v : val) (e : expr)  : expr :=
+    match e with
+    | Expr e => (SubstMap [(x, v)]) (Expr e)
+    | ClosedExpr f e Hfree =>
+      if bool_decide (x ∈ f) then (SubstMap ([(x, v)]) (ClosedExpr f e Hfree)) else ClosedExpr f e Hfree
+    | SubstMap xs e => if bool_decide (x ∈ xs.*1) then SubstMap xs e else
+                        SubstMap xs (subst x v e)
+    | Val v => Val v
+    | Var y => if bool_decide (x = y) then Val v else Var y
+    | Let y e1 e2 =>
+      Let y (subst x v e1) (if bool_decide (BNamed x ≠ y) then subst x v e2 else e2)
+    | UnOp op e => UnOp op (subst x v e)
+    | BinOp op e1 e2 => BinOp op (subst x v e1) (subst x v e2)
+    | If e0 e1 e2 => If (subst x v e0) (subst x v e1) (subst x v e2)
+    | While e0 e1 => While (subst x v e0) (subst x v e1)
+    | Pair e1 e2 => Pair (subst x v e1) (subst x v e2)
+    | Fst e => Fst (subst x v e)
+    | Snd e => Snd (subst x v e)
+    | InjL e => InjL (subst x v e)
+    | InjR e => InjR (subst x v e)
+    | Match e0 x1 e1 x2 e2 => Match (subst x v e0) x1 (if bool_decide (BNamed x ≠ x1) then subst x v e1 else e1)
+                                   x2 (if bool_decide (BNamed x ≠ x2) then subst x v e2 else e2)
+    | Fork e => Fork (subst x v e)
+    | AllocN e1 e2 => AllocN (subst x v e1) (subst x v e2)
+    | FreeN e1 e2 => FreeN (subst x v e1) (subst x v e2)
+    | Load o e => Load o (subst x v e)
+    | Store o e1 e2 => Store o (subst x v e1) (subst x v e2)
+    | CmpXchg e0 e1 e2 => CmpXchg (subst x v e0) (subst x v e1) (subst x v e2)
+    | FAA e1 e2 => FAA (subst x v e1) (subst x v e2)
+    | Call e1 e2 => Call (subst x v e1) (subst x v e2)
+    end.
+
+  Lemma to_expr_subst x v e :
+    to_expr (subst x v e) = simp_lang.subst x v (to_expr e).
+  Proof.
+    elim: e => /= [^ e].
+    all: (repeat case_decide => //=); f_equal; eauto.
+    - by rewrite -subst_map_subst subst_map_empty.
+    - by rewrite -subst_map_subst subst_map_empty.
+    - rewrite subst_free_vars //. set_solver.
+    - rewrite subst_free_vars // free_vars_subst_map dom_list_to_map. set_solver.
+    - revert select (to_expr _ = _) => ->.
+      rewrite subst_map_subst -subst_subst_map delete_notin //.
+      apply/not_elem_of_dom. rewrite dom_list_to_map. set_solver.
+  Qed.
+
+  Lemma tac_to_expr_subst x v e (P : _ → Prop) e':
+    (let ex := e' in subst x v e = ex) →
+    P (to_expr e') →
+    P (simp_lang.subst x v (to_expr e)).
+  Proof. by rewrite -to_expr_subst => ->. Qed.
+
+  Definition add_substmap (xs : list (string * val)) (e : expr) : expr :=
+    match xs with
+    | [] => e
+    | _ => SubstMap xs e
+    end.
+  Lemma to_expr_add_substmap xs e :
+    to_expr (add_substmap xs e) = subst_map (list_to_map xs) (to_expr e).
+  Proof. destruct xs => //=. by rewrite subst_map_empty. Qed.
+
+  Fixpoint combine_subst_map (xs : list (string * val)) (e : expr)  : expr :=
+    match e with
+    | SubstMap ys e => combine_subst_map (ys ++ xs) e
+    | Expr e => add_substmap xs $ Expr e
+    | ClosedExpr f e Hfree => add_substmap xs $ ClosedExpr f e Hfree
+    | Val v => add_substmap xs $ Val v
+    | Var y => add_substmap xs $ Var y
+    | Let y e1 e2 => add_substmap xs $
+      Let y (combine_subst_map [] e1) (combine_subst_map [] e2)
+    | UnOp op e => add_substmap xs $ UnOp op (combine_subst_map [] e)
+    | BinOp op e1 e2 => add_substmap xs $ BinOp op (combine_subst_map [] e1) (combine_subst_map [] e2)
+    | If e0 e1 e2 => add_substmap xs $ If (combine_subst_map [] e0) (combine_subst_map [] e1) (combine_subst_map [] e2)
+    | While e0 e1 => add_substmap xs $ While (combine_subst_map [] e0) (combine_subst_map [] e1)
+    | Pair e1 e2 => add_substmap xs $ Pair (combine_subst_map [] e1) (combine_subst_map [] e2)
+    | Fst e => add_substmap xs $ Fst (combine_subst_map [] e)
+    | Snd e => add_substmap xs $ Snd (combine_subst_map [] e)
+    | InjL e => add_substmap xs $ InjL (combine_subst_map [] e)
+    | InjR e => add_substmap xs $ InjR (combine_subst_map [] e)
+    | Match e0 x1 e1 x2 e2 => add_substmap xs $ Match (combine_subst_map [] e0) x1 (combine_subst_map [] e1)
+                                   x2 (combine_subst_map [] e2)
+    | Fork e => add_substmap xs $ Fork (combine_subst_map [] e)
+    | AllocN e1 e2 => add_substmap xs $ AllocN (combine_subst_map [] e1) (combine_subst_map [] e2)
+    | FreeN e1 e2 => add_substmap xs $ FreeN (combine_subst_map [] e1) (combine_subst_map [] e2)
+    | Load o e => add_substmap xs $ Load o (combine_subst_map [] e)
+    | Store o e1 e2 => add_substmap xs $ Store o (combine_subst_map [] e1) (combine_subst_map [] e2)
+    | CmpXchg e0 e1 e2 => add_substmap xs $ CmpXchg (combine_subst_map [] e0) (combine_subst_map [] e1) (combine_subst_map [] e2)
+    | FAA e1 e2 => add_substmap xs $ FAA (combine_subst_map [] e1) (combine_subst_map [] e2)
+    | Call e1 e2 => add_substmap xs $ Call (combine_subst_map [] e1) (combine_subst_map [] e2)
+    end.
+
+  Lemma to_expr_combine_subst_map xs e :
+    to_expr (combine_subst_map xs e) = subst_map (list_to_map xs) (to_expr e).
+  Proof.
+    elim: e xs => [^ e] /= xs; rewrite ?to_expr_add_substmap //=.
+    { revert select (∀ xs, _) => ->. by rewrite list_to_map_app subst_map_subst_map. }
+    all: do 2 f_equal.
+    all: repeat match goal with | H : ∀ xs, _ |- _ => specialize (H []) end.
+    all: etrans; [eassumption|] => /=; by rewrite subst_map_empty.
+  Qed.
+
+  Lemma to_expr_combine_subst_map_empty e :
+    to_expr (combine_subst_map [] e) = to_expr e.
+  Proof. by rewrite to_expr_combine_subst_map subst_map_empty. Qed.
+
+  Lemma tac_to_expr_combine_subst_map e (P : _ → Prop) e':
+    (let ex := e' in combine_subst_map [] e = ex) →
+    P (to_expr e') →
+    P (to_expr e).
+  Proof. move => <-. by rewrite to_expr_combine_subst_map_empty. Qed.
+
+  Definition binder_to_list (b : binder) : list string :=
+  match b with
+  | BNamed n => [n]
+  | BAnon => []
+  end.
+  Fixpoint free_vars (e : expr) : list string :=
+  match e with
+  | Expr _ => [] (* bogus but we don't care *)
+  | ClosedExpr f _ _ => f
+  | SubstMap xs e => (filter (λ v, v ∉ xs.*1) (free_vars e))
+  | Val v => []
+  | Var x => [x]
+  | Let x e1 e2 => free_vars e1 ++ (filter (λ v, v ∉ binder_to_list x) (free_vars e2))
+  | Match e0 x1 e1 x2 e2 =>
+    free_vars e0 ++
+    (filter (λ v, v ∉ binder_to_list x1) (free_vars e1)) ++
+    (filter (λ v, v ∉ binder_to_list x2) (free_vars e2))
+  | UnOp _ e | Fst e | Snd e | InjL e | InjR e | Fork e | Load _ e =>
+     free_vars e
+  | Call e1 e2 | While e1 e2 | BinOp _ e1 e2 | Pair e1 e2
+  | AllocN e1 e2 | FreeN e1 e2 | Store _ e1 e2 | FAA e1 e2 =>
+     free_vars e1 ++ free_vars e2
+  | If e0 e1 e2 | CmpXchg e0 e1 e2 =>
+     free_vars e0 ++ free_vars e1 ++ free_vars e2
+  end.
+
+  Fixpoint is_closed (free : list string) (e : expr) : bool :=
+  match e with
+  | Expr _ => false
+  | ClosedExpr f _ _ => bool_decide (f ⊆+ free)
+  | SubstMap xs e => is_closed (xs.*1 ++ free) e
+  | Val v => true
+  | Var x => bool_decide (x ∈ free)
+  | Let x e1 e2 => is_closed free e1 && is_closed (binder_to_list x ++ free) e2
+  | Match e0 x1 e1 x2 e2 =>
+    is_closed free e0 &&
+    is_closed (binder_to_list x1 ++ free) e1 &&
+    is_closed (binder_to_list x2 ++ free) e2
+  | UnOp _ e | Fst e | Snd e | InjL e | InjR e | Fork e | Load _ e =>
+     is_closed free e
+  | Call e1 e2 | While e1 e2 | BinOp _ e1 e2 | Pair e1 e2
+  | AllocN e1 e2 | FreeN e1 e2 | Store _ e1 e2 | FAA e1 e2 =>
+     is_closed free e1 && is_closed free e2
+  | If e0 e1 e2 | CmpXchg e0 e1 e2 =>
+     is_closed free e0 && is_closed free e1 && is_closed free e2
+  end.
+
+  Lemma to_expr_is_closed xs e:
+    is_closed xs e → parallel_subst.free_vars (to_expr e) ⊆ list_to_set xs.
+  Proof.
+    elim: e xs => [^ e] //= xs Hx.
+    all: destruct_and?.
+    all: repeat match goal with | H : (∀ xs, _) |- _ => specialize (H _ ltac:(done)) end.
+    { rewrite eHfree. set_unfold => ??. by apply: elem_of_submseteq. }
+    { revert select (_ ⊆ _). rewrite free_vars_subst_map list_to_set_app dom_list_to_map. set_solver. }
+    all: repeat match goal with | x : binder |- _ => destruct x end; set_solver.
+  Qed.
+
+  Lemma to_expr_is_closed_empty e:
+    is_closed [] e → parallel_subst.free_vars (to_expr e) = ∅.
+  Proof. move => /to_expr_is_closed. set_solver. Qed.
+
+End W.
+
+Ltac simpl_subst :=
+  repeat match goal with
+    | |- context C [subst ?x ?v ?e] =>
+      lazymatch e with
+      | subst _ _ _ => fail
+      | _ => idtac
+      end;
+      let e' := W.of_expr e in
+      let g := context C [subst x v (W.to_expr e')] in
+      change g;
+      pattern (simp_lang.subst x v (W.to_expr e'));
+      simple refine (W.tac_to_expr_subst _ _ _ _ _ _ _); [ shelve |
+      let ex := fresh "e" in intro ex; vm_compute; exact: eq_refl | ];
+      simple refine (W.tac_to_expr_combine_subst_map _ _ _ _ _); [ shelve |
+      let ex := fresh "e" in intro ex; vm_compute; exact: eq_refl | ];
+      simpl
+    end.
+Arguments subst : simpl never.
+
+Ltac solve_is_closed :=
+  lazymatch goal with
+  | |- free_vars ?e = ∅ =>
+    let e' := W.of_expr e in
+    apply (W.to_expr_is_closed_empty e');
+    vm_compute; exact: I
+  end.
+
+(*
+   Goal ∀ e : simp_lang.expr, free_vars e = list_to_set ["r"; "i" ] →
+    simp_lang.subst "r" (#0) (
+(* let: "r" := ref #0  in *)
+     let: "i" := ref #0  in
+     while: e do
+       "r" <- !"r" + !"m";;
+       (* Call ##f "x";; *)
+       "i" <- !"i" + #1
+     od;;
+     Free "i";;
+     let: "res" := !"r" in
+     Free "r";;
+     "res")%E = #0.
+     move => e?.
+     simpl_subst.
+   Abort.
+
+   Goal ∀ e : simp_lang.expr, free_vars e = list_to_set ["r"; "i" ] →
+    simp_lang.subst "i" (#0) (
+(* let: "r" := ref #0  in *)
+     (* let: "i" := ref #0  in *)
+while: subst_map (<["r":=#0]> ∅) e do #0 <- ! #0 + ! "m";; "i" <- ! "i" + #1 od ;;
+   simp_lang.FreeN #1 "i";; let: "res" := ! #0 in simp_lang.FreeN #1 #0;; "res")%E = #0.
+     move => ??.
+     simpl_subst.
+   Abort.
+
+  *)
